coq/ZF/Meta/Decl/Axiom/Union.v
@@ -11,12 +11,12 @@ Import ListNotations.
 (* forall a, exists b, forall x, x :< b <-> exists y, x :< y /\ y :< a          *)
 Definition Union : DeclP :=
   let concl :=
-      All VarTySet
-        (Ex VarTySet
-          (All VarTySet
+      All
+        (Ex
+          (All
             (Iff
               (Elem (Var 0) (Var 1))
-              (Ex VarTySet
+              (Ex
                 (And
                   (Elem (Var 1) (Var 0))
                   (Elem (Var 0) (Var 3)))))))
