coq/ZF/Meta/Test/Axiom/Specification.v
@@ -14,8 +14,9 @@ Require Import ZF.Meta.Decl.Axiom.Specification.
 Proposition Specification : CheckDeclP (Specification.env) Specification.
 Proof.
   (* Proof by Hermes + gpt 5.5                                                  *)
-  assert (CheckT Specification.env [] (conclP Specification) TyProp) as H1. {
-    apply CheckAll, CheckAll, CheckEx, CheckAll, CheckIff.
+  assert (CheckT Specification.env (ctxP Specification)
+    (conclP Specification) TyProp) as H1. {
+    apply CheckAll, CheckEx, CheckAll, CheckIff.
     - apply CheckElem; apply CheckVar; reflexivity.
     - apply CheckAnd.
       + apply CheckElem; apply CheckVar; reflexivity.
