coq/ZF/Meta/Ty.v
@@ -3,14 +3,3 @@ Inductive Ty : Type :=
 | TyClass : Ty
 | TyProp  : Ty
 .
-
-Inductive VarTy : Type :=
-| VarTySet   : VarTy
-| VarTyClass : VarTy
-.
-
-Definition toTy (vty:VarTy) : Ty :=
-  match vty with
-  | VarTySet   => TySet
-  | VarTyClass => TyClass
-  end.
